src/asn1/RIoT.Core.fst
@@ -14,7 +14,7 @@ module S = Spec.Hash.Definitions
 module H = Hacl.Hash.Definitions
 
 module ECDSA = Hacl.Impl.ECDSA
-module P256 = Hacl.Impl.P256
+// module P256 = Hacl.Impl.P256
 module Ed25519 = Hacl.Ed25519
 module Curve25519 = Hacl.Curve25519_51
 module HKDF = Hacl.HKDF
@@ -34,192 +34,130 @@ open RIoT.Declassify
 
 module B32 = FStar.Bytes
 
-#set-options "--query_stats --z3rlimit 16 --initial_fuel 8 --initial_ifuel 2"
+#set-options "--query_stats --z3rlimit 16"
 let _ = assert (length_of_oid OID_EC_GRP_SECP256R1 == 6)
 
-// let salt_len: a:size_t{(v a) > 0 /\ Spec.Agile.HMAC.keysized alg (v a)}
-//   = 32ul
-// (* ZT: Hacl.HKDF.fsti and Spec.Agile.HKDF.fsti
-//        have different spec, I choose the smaller
-//        one `pow2 32` here*)
-// let info_len: a:size_t{(v a) > 0 /\ hash_length SHA2_256 + v a + 1 + block_length SHA2_256 <= pow2 32}
-//   = 32ul
-// let okm_len : a:size_t{(v a) > 0}
-//   = 32ul
+// #push-options "--z3rlimit 32"
+// let label_DeviceID_l: list byte_sec = [u8 0; u8 0]
+// let label_DeviceID_len
+// : len: size_t { valid_hkdf_lbl_len len /\
+//                 v len == List.length label_DeviceID_l }
+// = assert_norm (valid_hkdf_lbl_len 2ul);
+//   assert_norm (List.length label_DeviceID_l == 2);
+//   2ul
+// let label_DeviceID
+// : ib:IB.libuffer uint8 (v label_DeviceID_len) (Seq.createL label_DeviceID_l)
+//   { IB.frameOf ib == HS.root /\ IB.recallable ib /\
+//     valid_hkdf_lbl_len (B.len ib) }
+// = assert_norm (valid_hkdf_lbl_len label_DeviceID_len);
+//   IB.igcmalloc_of_list HS.root label_DeviceID_l
 
+// let label_AliasKey_l: list byte_sec = [u8 1; u8 1]
+// let label_AliasKey_len
+// : len: size_t { valid_hkdf_lbl_len len /\
+//                 v len == List.length label_AliasKey_l }
+// = assert_norm (valid_hkdf_lbl_len 2ul);
+//   assert_norm (List.length label_AliasKey_l == 2);
+//   2ul
+// let label_AliasKey
+// : ib:IB.libuffer uint8 (v label_AliasKey_len) (Seq.createL label_AliasKey_l)
+//   { IB.frameOf ib == HS.root /\ IB.recallable ib /\
+//     valid_hkdf_lbl_len (B.len ib) }
+// = assert_norm (valid_hkdf_lbl_len label_AliasKey_len);
+//   IB.igcmalloc_of_list HS.root label_AliasKey_l
+// #push-options
 
-#push-options "--z3rlimit 32"
-let riot_label_DeviceID: ib:IB.libuffer uint8 2 (Seq.createL [u8 0; u8 0])
-                         { IB.frameOf ib == HS.root /\
-                           IB.recallable ib /\
-                           valid_hkdf_lbl_len (B.len ib) }
-= assert_norm (valid_hkdf_lbl_len 2ul);
-  IB.igcmalloc_of_list HS.root [u8 0; u8 0]
-
-let riot_label_AliasKey: ib:IB.libuffer uint8 2 (Seq.createL [u8 1; u8 1])
-                         { IB.frameOf ib == HS.root /\
-                           IB.recallable ib /\
-                           valid_hkdf_lbl_len (B.len ib) }
-= assert_norm (valid_hkdf_lbl_len 2ul);
-  IB.igcmalloc_of_list HS.root [u8 1; u8 1]
-#push-options
-// assume val s: Seq.lseq uint8 3
-// let x: B32.lbytes32 3ul = B32.hide s
-
-
+unfold
 let valid_ed25519_sign_mag_length
   (l: nat)
 = 64 + l <= max_size_t
 
 #restart-solver
-#push-options "--query_stats --z3rlimit 32 --fuel 4 --ifuel 2"
+#push-options "--query_stats --z3rlimit 256 --fuel 8 --ifuel 4"
 let riot_main
-  (cdi : B.lbuffer uint8 32)
-  (fwid: B.lbuffer uint8 32)
-  (riot_version: datatype_of_asn1_type INTEGER)
-  (aliasKey_crt_len: size_t)
-  (aliasKey_crt_pos: size_t)
-  (aliasKey_crt: B.lbuffer pub_uint8 (v aliasKey_crt_len))
-  (aliasKey_pub: B.lbuffer pub_uint8 32)
+(* inputs *)
+  (cdi : B.lbuffer byte_sec 32)
+  (fwid: B.lbuffer byte_sec 32)
+  (version: datatype_of_asn1_type INTEGER)
+  (aliasKeyTBS_template_len: size_t)
+  (aliasKeyTBS_template: B.lbuffer byte_pub (v aliasKeyTBS_template_len))
+  (deviceID_label_len: size_t)
+  (deviceID_label: B.lbuffer byte_sec (v deviceID_label_len))
+  (aliasKey_label_len: size_t)
+  (aliasKey_label: B.lbuffer byte_sec (v deviceID_label_len))
+(* outputs *)
+  (aliasKeyCRT_len: size_t)
+  (aliasKeyCRT: B.lbuffer byte_pub (v aliasKeyCRT_len))
+  (aliasKey_pub: B.lbuffer byte_pub 32)
   (aliasKey_priv: B.lbuffer uint8 32)
 : HST.Stack unit
   (requires fun h ->
     B.(all_live h [buf cdi;
                    buf fwid;
+                   buf aliasKeyTBS_template;
+                   buf deviceID_label;
+                   buf aliasKey_label;
+                   buf aliasKeyCRT;
                    buf aliasKey_pub;
-                   buf aliasKey_priv;
-                   buf aliasKey_crt]) /\
+                   buf aliasKey_priv]) /\
     B.(all_disjoint [loc_buffer cdi;
                      loc_buffer fwid;
+                     loc_buffer aliasKeyTBS_template;
+                     loc_buffer deviceID_label;
+                     loc_buffer aliasKey_label;
+                     loc_buffer aliasKeyCRT;
                      loc_buffer aliasKey_pub;
-                     loc_buffer aliasKey_priv;
-                     loc_buffer aliasKey_crt]) /\
-    (* pre *) 0 <= v aliasKey_crt_pos /\ v aliasKey_crt_pos <= v aliasKey_crt_len /\
-   (let deviceID_pub, deviceID_priv = riot_derive_DeviceID_spec
-                                        (B.as_seq h cdi)
-                                        (B.len riot_label_DeviceID)
-                                        (B.as_seq h riot_label_DeviceID) in
-    let aliasKey_pub, aliasKey_priv = riot_derive_AliasKey_spec
-                                        (B.as_seq h cdi)
-                                        (B.as_seq h fwid)
-                                        (B.len riot_label_AliasKey)
-                                        (B.as_seq h riot_label_AliasKey) in
-    let            aliasKey_crt_tbs = x509_get_aliasKey_crt_tbs_spec
-                                        (B.as_seq h cdi)
-                                        (B.as_seq h fwid)
-                                        (riot_version)
-                                        (deviceID_pub)
-                                        (aliasKey_pub)
-                                        (aliasKey_crt_len)
-                                        (aliasKey_crt_pos)
-                                        (B.as_seq h aliasKey_crt) in
-     (* `aliasKey_crt_tbs` has an Ed25519 signable length -- pre condition for `aliasKey_crt_pos` *)
-     (* pre *) valid_ed25519_sign_mag_length (Seq.length aliasKey_crt_tbs) /\
-    (let               aliasKey_crt = x509_get_aliasKey_crt_spec
-                                        (deviceID_priv)
-                                        (aliasKey_crt_tbs) in
-     (* `aliasKey_crt` buffer has enough space *)
-     (* pre *) Seq.length aliasKey_crt <= - v aliasKey_crt_pos )))
-   (ensures fun h0 _ h1 -> True)
-= ()
+                     loc_buffer aliasKey_priv]) /\
+   valid_hkdf_lbl_len deviceID_label_len /\
+   valid_hkdf_lbl_len aliasKey_label_len /\
+   valid_aliasKeyTBS_ingredients aliasKeyTBS_template_len version /\
+   valid_aliasKeyCRT_ingredients (len_of_AliasKeyTBS aliasKeyTBS_template_len version) /\
+   v aliasKeyCRT_len == length_of_AliasKeyCRT (len_of_AliasKeyTBS aliasKeyTBS_template_len version)
+   )
+   (ensures fun h0 _ h1 ->
+     B.(modifies (loc_buffer aliasKeyCRT `loc_union` loc_buffer aliasKey_pub `loc_union` loc_buffer aliasKey_priv) h0 h1)
+   )
+= HST.push_frame ();
 
-let () = ()
+(* Allocate DeviceID *)
+  let deviceID_pub : B.lbuffer byte_pub 32 = B.alloca 0x00uy    32ul in
+  let deviceID_priv: B.lbuffer byte_sec 32 = B.alloca (u8 0x00) 32ul in
 
-(*)
-#restart-solver
-#push-options "--query_stats --z3rlimit 256 --initial_fuel 8 --max_fuel 8 --initial_ifuel 4"
-let riot_main
-  (cdi : B.lbuffer uint8 32)
-  (fwid: B.lbuffer uint8 32)
-  (riot_version: datatype_of_asn1_type INTEGER)
-  (aliasKey_crt_len: size_t)
-  (aliasKey_crt_pos: size_t)
-  (aliasKey_crt: B.lbuffer pub_uint8 (v aliasKey_crt_len))
-  (aliasKey_pub: B.lbuffer pub_uint8 32)
-  (aliasKey_priv: B.lbuffer uint8 32)
-: HST.Stack unit
-  (requires fun h ->
-    B.(all_live h [buf cdi;
-                   buf fwid;
-                   buf aliasKey_pub;
-                   buf aliasKey_priv;
-                   buf aliasKey_crt]) /\
-    B.(all_disjoint [loc_buffer cdi;
-                     loc_buffer fwid;
-                     loc_buffer aliasKey_pub;
-                     loc_buffer aliasKey_priv;
-                     loc_buffer aliasKey_crt]) /\
-    0 <= v aliasKey_crt_pos /\ v aliasKey_crt_pos <= v aliasKey_crt_len /\
-    v aliasKey_crt_len + 64 <= max_size_t /\
-   (let cdigest = Spec.Agile.Hash.hash alg (B.as_seq h cdi) in
-    let deviceID_pub, deviceID_priv = riot_derive_key_pair_spec 32ul cdigest 2ul (B.as_seq h riot_label_DeviceID) in
-    let adigest = Spec.Agile.HMAC.hmac alg cdigest (B.as_seq h fwid) in
-    let aliasKey_pub, aliasKey_priv = riot_derive_key_pair_spec 32ul adigest 2ul (B.as_seq h riot_label_DeviceID) in
-    let deviceID_pub32: B32.lbytes32 32ul = B32.hide deviceID_pub in
-    let fwid32: B32.lbytes32 32ul = B32.hide (declassify_secret_bytes 32 (B.as_seq h fwid)) in
-    let riot_extension = x509_get_riot_extension riot_version deviceID_pub32 fwid32 in
-    let riot_extension_sx = serialize_x509_extension_sequence_TLV serialize_compositeDeviceID_sequence_TLV
-                            `serialize`
-                            riot_extension in
-    (* AliasKey Certificate TBS *)
-    let aliasKey_crt_tbs = Seq.slice (B.as_seq h aliasKey_crt) 0 (v aliasKey_crt_pos)
-                           `Seq.append` (* FIXME: Here, we need to require that `tbs`'s length is acceptable by the signing fun *)
-                           riot_extension_sx in
-    let _ = lemma_serialize_x509_extension_size serialize_compositeDeviceID_sequence_TLV riot_extension;
-            (**) lemma_serialize_asn1_oid_TLV_size riot_extension.x509_extID;
-            (**) lemma_serialize_asn1_boolean_TLV_size riot_extension.x509_extCritical;
-            (**) lemma_serialize_compositeDeviceID_sequence_TLV_size_exact riot_extension.x509_extValue;
-            lemma_serialize_x509_extension_sequence_TLV_size serialize_compositeDeviceID_sequence_TLV riot_extension in
-    let aliasKey_crt_tbs = classify_public_bytes (Seq.length aliasKey_crt_tbs) aliasKey_crt_tbs in
-    Seq.length aliasKey_crt_tbs + 64 <= max_size_t /\
-   (let aliasKey_crt_sig = Spec.Ed25519.sign deviceID_priv aliasKey_crt_tbs in
-    let aliasKey_crt_sig32: B32.lbytes32 64ul = B32.hide (declassify_secret_bytes 64 aliasKey_crt_sig) in
-    let aliasKey_crt_sig_bs = {bs_len = 65ul; bs_unused_bits = 0ul; bs_s = aliasKey_crt_sig32} in
-    (* AliasKey Certificate Signature *)
-    // let aliasKey_crt_sig_sx = (OID_EC_ALG_UNRESTRICTED (*FIXME*) `serialize_envelop_OID_with` serialize_asn1_bit_string_TLV)
-    //                           `serialize`
-    //                           (lemma_serialize_asn1_bit_string_TLV_size aliasKey_crt_sig_bs;
-    //                            (OID_EC_ALG_UNRESTRICTED, aliasKey_crt_sig_bs)) in
-    v aliasKey_crt_len - v aliasKey_crt_pos >= 50)))
-    // length_of_opaque_serialization serialize_compositeDeviceID_sequence_TLV (x509_get_compositeDeviceID) ))
-  (ensures  fun h0 _ h1 ->
-    True)
-= admit() (*)
-  HST.push_frame ();
-  let cdi = HW.get_cdi st in
-  let cDigest: b:B.buffer uint8{B.length b == v digest_len} = B.alloca (u8 0) digest_len in
-  (**)assert_norm (v digest_len <= max_input_length alg);
-  riot_hash alg
-    cdi cdi_len    //in : data
-    cDigest;       //out: digest
-  let deviceID_private_key: b:B.buffer uint8{B.length b == v digest_len} = B.alloca (u8 0) digest_len in
-  (**)assert_norm (v digest_len + block_length alg <= max_input_length alg);
-  riot_derive_key_pair
-    rout.deviceID_public_key //out: public key
-    deviceID_private_key     //out: private key
-    cDigest digest_len;      //in :ikm
+(* Derive DeviceID *)
+  derive_DeviceID
+    (* pub *) deviceID_pub
+    (* priv*) deviceID_priv
+    (* cdi *) cdi
+    (* lbl *) deviceID_label_len deviceID_label;
 
-  (* NOTE: Now I just fill the public key into the To-Be-Signed region *)
-  B.blit
-    rout.deviceID_public_key 0ul
-    rout.deviceID_cert.tbs   0ul
-    32ul;
-  Ed25519.sign
-    rout.deviceID_cert.sig  //out: signature
-    deviceID_private_key    //in : secret
-    32ul                    //in : msglen
-    rout.deviceID_cert.tbs; //in : msg
+(* Derive AliasKey *)
+  derive_AliasKey
+    (* pub *) deviceID_pub
+    (* priv*) deviceID_priv
+    (* cdi *) cdi
+    (* fwid*) fwid
+    (* lbl *) deviceID_label_len deviceID_label;
 
-  (* FIXME: just consider deviceID now *)
-  // (* NOTE: hmac requires disjointness *)
-  // let cfDigest: b:B.buffer uint8{B.length b == v digest_len} = B.alloca (u8 0) digest_len in
-  // riot_hmac alg
-  //   cfDigest            //out: tag
-  //   cDigest digest_len  //in : key
-  //   fwid    digest_len; //in : data
-  // riot_derive_key_pair
-  //   rout.alias_public_key  //out: public key
-  //   rout.alias_private_key //out: private key
-  //   cfDigest digest_len;   //in :ikm
+(* Create AliasKeyTBS *)
+  let aliasKeyTBS_len: asn1_TLV_int32_of_type SEQUENCE = len_of_AliasKeyTBS aliasKeyTBS_template_len version in
+  let aliasKeyTBS: B.lbuffer byte_pub (v aliasKeyTBS_len) = B.alloca 0x00uy aliasKeyTBS_len in
+  create_aliasKeyTBS
+    (* fwid   *) fwid
+    (* version*) version
+    (*deviceID*) deviceID_pub
+    (*aliasKey*) aliasKey_pub
+    (*template*) aliasKeyTBS_template_len
+                 aliasKeyTBS_template
+    (*   tbs  *) aliasKeyTBS_len
+                 aliasKeyTBS;
 
-  HST.pop_frame ()
+(* Sign AliasKeyTBS and Finalize AliasKeyCRT*)
+  sign_and_finalize_aliasKeyCRT
+    (*signing key*) deviceID_priv
+    (*AliasKeyTBS*) aliasKeyTBS_len
+                    aliasKeyTBS
+    (*AliasKeyCRT*) aliasKeyCRT_len
+                    aliasKeyCRT;
+
+  HST.pop_frame()
+#pop-options
